Advent of code

src/Parsers/examples/ParserGenerator.dfy
@@ -3,9 +3,9 @@
 include "../stringParsersBuilders.dfy"
 
 // A small regex-like language that can be turned into a straightforward parser
-// a compiler from this language to an imperative language
-// and a parser that can act 
-// and a parser that can act as a specification
+// So first we parse the parser to ParserSpec, we convert it to a parser
+// and we parse the string using this parser.
+// TODO: Compile this parser and prove it does the same.
 module ParserGenerator {
   import opened StringParsersBuilders
 
@@ -21,12 +21,19 @@ module ParserGenerator {
     | Or(left: ParserSpec, right: ParserSpec)
     | Repeat(p: ParserSpec)
   {
+    predicate OnlyAndRepeat() {
+      match this
+      case Const(s) => true
+      case And(left, right) => left.OnlyAndRepeat() && right.OnlyAndRepeat()
+      case Or(left, right) => false
+      case Repeat(p) => p.OnlyAndRepeat()
+    }
     function ToParser(): B<bool> {
       match this
       case Const(s) => S(s).M(ToBool())
       case And(left, right) => left.ToParser().e_I(right.ToParser()).M(ToBool())
       case Or(left, right) => O([left.ToParser().??(), right.ToParser()]).M(ToBool())
-      case Repeat(x) => x.ToParser().ZeroOrMore().M(ToBool())
+      case Repeat(x) => x.ToParser().??().ZeroOrMore().M(ToBool())
     }
     function ToString(): string {
       match this
@@ -66,4 +73,94 @@ module ParserGenerator {
     program := "abcdeml";
     print underlying.apply(program); // Should print true
   }
+
+  // TODO: Some kind of compilation?
+/*
+  datatype ParserStmt = 
+      Expect(c: char)
+    | Stmts(first: ParserStmt, next: PArserStmt)
+    | Repeat(underlying: ParserStmt)
+    | Break()
+  {
+    function ToProgram(indent: string := ""): string {
+      match this {
+        case Expect(c) => "if input[i] == '" + [c] + "' { }"
+      }
+    }
+    // (ok, cancelling)
+    function Run(input: string, index: nat): (bool, nat) {
+      if |input| <= index then (false, index) else
+      match this {
+        case Expect(c) => (input[index] == c, index + 1)
+        case Stmts(first) =>
+          if s == [] then (true, index)
+          else 
+            var (r, newIndex) := !s[0].Run(input, index);
+            if r then Stmts(s[1..]).Run(input, newIndex)
+            else (false, index) // We completely forget about the failure
+        case Break() => 
+        case Repeat(stmts) =>
+          stmts 
+      }
+    }
+
+    method RunImperative(input: string) returns (b: bool)
+      ensures b == Run(input, 0)
+    {
+      var i := 
+    }
+  }
+  //datatype 
+*/
+  // A ParserSpec can be compiled to this non-deterministic Automata
+  // We will prove that the two parsing strategies are equivalent
+  /*datatype Automata = Automata(
+    nStates: nat,
+    startState: nat,
+    transitions: set<(nat, char, nat)>,
+    finalState: set<nat>
+  )
+  {
+    static function FromParserSpec(spec: ParserSpec): Automata {
+      match spec {
+        case Const("") =>
+          Automata(1, 0, {}, {0})
+        case Const(s) =>
+          var a := FromParserSpec(Const(s[1..]));
+          var newStart := a.nStates;
+          Automata(a.nStates + 1, newStart, a.transitions + {(newStart, s[0], a.startState)}, a.finalState)
+        case Or(left, right) =>
+          var l := FromParserSpec(left);
+          var r := FromParserSpec(right);
+          var offsetRight := (n: nat) => n + l.nStates;
+          var newStart := l.nStates + r.nStates + 1;
+          var rightTransitions := set rt <- r.transitions :: (offsetRight(rt.0), rt.1, offsetRight(rt.2));
+          Automata(l.nStates + r.nStates + 1,
+            newStart,
+            l.transitions + rightTransitions +
+            + set firstLeftTransition <- l.transitions |
+                firstLeftTransition.0 == l.start
+          )
+        case _ => Automata(0, 0, {}, {})
+      }
+    }
+
+    function Run(input: string, states: set<nat>, index: nat): set<nat> {
+      if index >= |input| then {}
+      else set newState: nat, s: nat |
+              0 <= newState < nStates && 0 <= s < nStates &&
+              (s, input[index], newState) in transitions
+        :: newState 
+    }
+    predicate Accepts(input: string) {
+      Run(input, {startState}, 0) * finalState != {}
+    }
+
+    lemma Equivalence(spec: ParserSpec, input: string)
+      ensures spec.ToParser().apply(input).Success?
+              <==> FromParserSpec(spec).Accepts(input)
+    {
+      
+    }
+  }*/
 }
