src/Parsers/examples/AdventOfCode1.dfy
@@ -1,0 +1,36 @@
+// RUN: %test "%s"
+
+include "../stringParsersBuilders.dfy"
+
+// A small regex-like language that can be turned into a straightforward parser
+// So first we parse the parser to ParserSpec, we convert it to a parser
+// and we parse the string using this parser.
+// TODO: Compile this parser and prove it does the same.
+module AdventOfCode1 {
+  import opened StringParsersBuilders
+
+  const nonDigit :=
+    Except("0123456789\r\n").ZeroOrMore()
+
+  const digit :=
+    B(P.DigitNumber())
+
+  const parseLine :=
+    nonDigit.e_I(digit).Bind((first: nat) =>
+      nonDigit.e_I(digit).??().Rep((first, first),
+        (pair: (nat, nat), newDigit: nat) => (pair.0, newDigit)
+      )).I_e(nonDigit)
+      
+  const parseInput :=
+    parseLine.I_e(S("\r").?().e_I(S("\n").?()))
+      .Rep(0, (acc: int, newElem: (nat, nat)) =>
+      acc + newElem.0 * 10 + newElem.1)
+
+  method {:test} TestParser() {
+    var input := @"1abc2
+pqr3stu8vwx
+a1b2c3d4e5f
+treb7uchet";
+    ParseTest(parseInput, input);
+  }
+}
